

\myProblems[Solve these cube root equations.]
{
    $\myRoot[3]{x-4} - 15 = -20$
    %   root3(x-4) = -5 
    %   x-4 = -125
    %   x = -121
}
{
    $4\myRoot[3]{2x-3} + 8 = 20$
    % 4 root3(2x-3) = 12 
    %   root3(2x-3) = 3
    %   2x-3 = 27
    %   2x = 30 
    %   x = 15
}{2.2in}[\raggedleft\gap{$x=-121$}][\raggedleft\gap{$x=15$}]




\myProblems
{
    $\myRoot[3]{3x-2}  = \myRoot[3]{2x+19}$
    % 3x-2 = 2x+19 
    % x-2 = 19
    % x = 21
}
{
    $\myRoot[3]{x} - 4x = 0$
    % root3(x) = 4x
    % x = 64x^3 
    % 0 = 64x^3 - x 
    % 0 = x( 64x^2 - 1 )
    % 0 = x (8x - 1) (8x + 1)
}{2.2in}[\raggedleft\gap{$x=21$}][\raggedleft\gap{$x=0,\frac{1}{8},-\frac{1}{8}$}]




\myWideProblem
{
    $\myRoot[3]{x^2 + 2x + 61 } = 4$
    % x^2 + 2x + 61 = 4^3 
    % x^2 + 2x + 61 = 64 
    % x^2 + 2x - 3 = 0 
    % (x+3)(x-1) = 0
}{1in}[\raggedleft\gap{$x=1,-3$}]
