\section*{The Zero Product Property}

Sometimes we are given equations in that are already \gap{factored} and equal to \gap{zero}.
Here are some examples:
\begin{taggedblock}{on-level}
    \begin{align*}
        x\,(x+4)     &= 0  \\
        (x+1)(x+4)  &= 0  \\
        (x+1)(x-4)  &= 0  \\
        (3x+1)(x-4) &= 0  \\
    \end{align*}
\end{taggedblock}
\begin{taggedblock}{pre-AP}
    \begin{align*}
        x\,(x+4)     &= 0  \\
        (x-1)(x+4)  &= 0  \\
        (2x+1)(13x-5) &= 0  \\
        (5x+\frac{1}{2})(x-3) &= 0 \\
        (5x-7)(x-4)(5x-2) &= 0 \\
    \end{align*}
\end{taggedblock}

Already-factored equations like this  
are easy to solve.

\begin{myConceptSteps}{
    To solve factored equations that are equal to zero\dots
}
\myStep{split}{
    Separately set each factor to zero. This will give you several simpler equations.
}
\myStep{solve}{
    Solve each of the simpler equations.
}
\myStep{collect}{
    The final answer is all of the separate solutions.
}
\end{myConceptSteps}

\begin{center}
    \begin{tcolorbox}[width=5in]
        This only works if one side of the equation 
        {\bfseries\itshape equals} \gap{zero}.
    \end{tcolorbox}
\end{center}

\begin{taggedblock}{on-level}
    \myBlankExample{1.5in}{
        Solve this factored equation using the zero product property:
        \[
            (x-2)(x-3) = 0
        \]
    }
    \myBlankExample{1.5in}{
        Solve this factored equation using the zero product property:
        \[
            3x (x+7) = 0
        \]
    }
    
    \myBlankExample{1.5in}{
        Solve this factored equation using the zero product property:
        \[
            (2x + 7) (3x - 4) = 0
        \]
    }
\end{taggedblock}


\begin{taggedblock}{pre-AP}
    \myBlankExample{1.5in}{
        Solve this factored equation using the zero product property:
        \[
            (x + 3) (5x - 10) = 0
        \]
    }

    \myBlankExample{1.5in}{
        Solve this factored equation using the zero product property:
        \[
            \frac{2}{3}x (9x - 5) = 0
        \]
    }
    
    \myBlankExample{2.5in}{
        Solve this factored equation using the zero product property:
        \[
            ( x-8) (2x - 8)(3x - 5) = 0
        \]
    }
\end{taggedblock}
            