% \subsection{Zero and Negative Exponents}
\begin{tcbraster}[
    raster columns = 2,
    raster equal height,
    colback = white,
    % raster left skip = 0.75in, raster right skip = 0.75in, raster column skip = 0.75in,
    raster before skip = 0in, raster after skip = 0in,
]
\begin{tcolorbox}[]
    {\bfseries Zero Exponent Rule.}
    Any base raised to the zero power is equal to one.
    \[b^0 = 1\]
\end{tcolorbox}
\begin{tcolorbox}[]
    {\bfseries Negative Exponent Rule.}
    If a factor in a fraction is moved across the fraction bar,
    then the sign of its exponent is changed.
    \begin{align*}
       b^{-m} &= \frac{1}{b^m}     &\frac{1}{b^{-m}}&=b^m \\
    \end{align*}
    \vspace{-1\onelineskip}
\end{tcolorbox}

\begin{tcolorbox}[enhanced,opacityframe=0,]
    \begin{itemize}
        \item $2^0 = 1$
        \item $x^0 = 1$
        \item $\left(3x^2 y^{-3}\right)^0 = 1$
    \end{itemize}
    \end{tcolorbox}
\begin{tcolorbox}[enhanced,opacityframe=0,]
    \begin{itemize}
        \item $x^{-1} = \frac{1}{x}$
        \item $2^{-3} = \frac{1}{2^3} = \frac{1}{8}$
        \item $
            \left(\frac{x^3y^{-4}}{z^{-2}}\right) 
            = 
            \left(\frac{x^3z^2}{y^4}\right) 
            $
    \end{itemize}
\end{tcolorbox}

\end{tcbraster}


